[Civl] Fix reserve example (#574)
* first working version

* some cleanup

* added golden file

* some cleanup

Test/civl/reserve.bpl
@@ -1,157 +1,175 @@
+// RUN: %parallel-boogie "%s" > "%t"
+// RUN: %diff "%s.expect" "%t"
+
+/*
+This example models a memory allocator based on count of free cells (freeSpace) and an
+array that keeps tracks of the allocation status of each cell (isFree). To allocate
+a cell, freeSpace is decremented atomically, blocking to ensure that freeSpace does not
+go below zero. If the decrement succeeds, then a scan of isFree is performed to find a
+free cell. The goal of the verification is to prove that this scan will succeed. The
+main challenge in the proof is to reason about cardinality of constructed sets.
+*/
+
+type {:linear "tid"} Tid = int;
+
 const memLo: int;
 const memHi: int;
 axiom 0 < memLo && memLo <= memHi;
-function memAddr(i:int) returns (bool) { memLo <= i && i < memHi }
+function {:inline} memAddr(i: int) returns (bool) { memLo <= i && i < memHi }
 
-const numMutators: int;
-axiom 0 < numMutators;
-function {:inline} mutatorAddr(i: int) returns (bool) { 1 <= i && i <= numMutators }
+type {:datatype} Bijection;
+function {:constructor} Bijection(domain: [Tid]bool, range: [int]bool, tidToPtr: [Tid]int, ptrToTid: [int]Tid): Bijection;
 
-const GcTid: int;
-axiom GcTid > numMutators;
-
-function {:inline} Subset(X: [int]bool, Y: [int]bool) : (bool)
-{
-    MapOr(MapNot(X), Y) == MapConst(true)
-}
-
-type {:linear "tid"} X = int;
-
-var {:layer 0,1} Free: [int]bool;
+var {:layer 0,1} isFree: [int]bool;
 var {:layer 0,1} freeSpace: int;
-var {:layer 0,1} AllocatingAtOrAfter: [int][X]bool;
-var {:layer 0,1} NumFreeAtOrAfter: [int]int;
+var {:layer 0,1} allocMap: Bijection;
 
-function Size([int]bool) returns (int);
-axiom (forall X: [int]bool :: 0 <= Size(X));
-axiom (forall X: [int]bool, x: int :: X[x] ==> 1 <= Size(X));
-axiom (forall X: [int]bool, x: int :: X[x] ==> X[x:=true] == X);
-axiom (forall X: [int]bool, x: int :: !X[x] ==> X[x:=false] == X);
-axiom (forall X: [int]bool, x: int :: Size(X[x := false]) + 1 == Size(X[x := true]));
-axiom (forall X, Y: [int]bool :: Subset(X, Y) ==> Size(X) < Size(Y) || X == Y);
-
-function {:inline} Invariant(NumFreeAtOrAfter: [int]int, AllocatingAtOrAfter: [int][X]bool, Free: [int]bool, freeSpace: int) : (bool)
-{
-    Size(AllocatingAtOrAfter[memLo]) + freeSpace == NumFreeAtOrAfter[memLo] &&
-    (forall u: int :: Size(AllocatingAtOrAfter[u]) <= NumFreeAtOrAfter[u]) &&
-    0 <= freeSpace &&
-    (forall u: int, v: int :: memAddr(u) && memAddr(v) && u <= v ==> Subset(AllocatingAtOrAfter[v], AllocatingAtOrAfter[u])) &&
-    (forall u: int :: memAddr(u) || NumFreeAtOrAfter[u] == 0) &&
-    (forall u: int :: {memAddr(u)} memAddr(u) ==> NumFreeAtOrAfter[u] == (NumFreeAtOrAfter[u+1] + (if Free[u] then 1 else 0)))
+function {:inline} BijectionInvariant(allocMap: Bijection): bool {
+    (forall tid: Tid ::
+        domain#Bijection(allocMap)[tid] ==>
+            range#Bijection(allocMap)[tidToPtr#Bijection(allocMap)[tid]] &&
+            ptrToTid#Bijection(allocMap)[tidToPtr#Bijection(allocMap)[tid]] == tid)
+    &&
+    (forall ptr: int ::
+        range#Bijection(allocMap)[ptr] ==>
+            domain#Bijection(allocMap)[ptrToTid#Bijection(allocMap)[ptr]] &&
+            tidToPtr#Bijection(allocMap)[ptrToTid#Bijection(allocMap)[ptr]] == ptr)
 }
 
-procedure {:yields} {:layer 0,1} DecrementFreeSpace({:cnst "tid"} tid: X);
-ensures {:atomic} |{ A:   assert AllocatingAtOrAfter[memLo] == AllocatingAtOrAfter[memLo][tid := false];
-                          assume 0 < freeSpace;
-                          freeSpace := freeSpace - 1;
-                          AllocatingAtOrAfter[memLo][tid] := true;
-                          return true; }|;
+procedure {:yield_invariant} {:layer 1} YieldInvariant();
+requires 0 <= freeSpace;
+requires BijectionInvariant(allocMap);
+requires (forall y: int :: isFree[y] ==> memAddr(y));
+requires MapDiff(range#Bijection(allocMap), isFree) == MapConst(false);
+requires freeSpace == Size(MapDiff(isFree, range#Bijection(allocMap)));
 
-procedure {:yields} {:layer 0,1} AllocIfPtrFree({:cnst "tid"} tid:int, ptr:int) returns (spaceFound:bool);
-ensures {:atomic} |{
-    A: assert memAddr(ptr);
-       assert Free[ptr] || memAddr(ptr + 1);
-       assert (forall u: int :: AllocatingAtOrAfter[u][tid] <==> memLo <= u && u <= ptr);
-       spaceFound := Free[ptr];
-       goto B, C;
-    B: assume (spaceFound);
-       Free[ptr] := false;
-       NumFreeAtOrAfter := (lambda u: int :: NumFreeAtOrAfter[u] - (if memLo <= u && u <= ptr then 1 else 0));
-       AllocatingAtOrAfter := (lambda u: int :: AllocatingAtOrAfter[u][tid := false]);
-       return true;
-    C: assume (!spaceFound);
-       AllocatingAtOrAfter[ptr+1][tid] := true;
-       return true; }|;
+function Size<T>([T]bool) returns (int);
 
-procedure {:yields} {:layer 0,1} Reclaim({:cnst "tid"} tid:int);
-ensures {:atomic} |{ var ptr: int;
-    A: assume memAddr(ptr) && !Free[ptr];
-       freeSpace := freeSpace + 1;
-       Free[ptr] := true;
-       NumFreeAtOrAfter := (lambda u: int :: NumFreeAtOrAfter[u] + (if memLo <= u && u <= ptr then 1 else 0));
-       return true; }|;
+procedure {:lemma} SizeLemma1<T>(X: [T]bool, x: T);
+ensures Size(X[x := false]) + 1 == Size(X[x := true]);
 
-procedure {:yields} {:layer 1} YieldAlloc({:cnst "tid"} tid:int, i: int)
-requires {:layer 1} mutatorAddr(tid);
-requires {:expand} {:layer 1} Invariant(NumFreeAtOrAfter, AllocatingAtOrAfter, Free, freeSpace);
-requires {:layer 1} (forall u: int :: AllocatingAtOrAfter[u][tid] <==> memLo <= u && u <= i);
-ensures {:layer 1} Invariant(NumFreeAtOrAfter, AllocatingAtOrAfter, Free, freeSpace);
-ensures {:layer 1} (forall u: int :: AllocatingAtOrAfter[u][tid] <==> memLo <= u && u <= i);
+procedure {:lemma} SizeLemma2<T>(X: [T]bool, Y: [T]bool);
+requires MapDiff(X, Y) == MapConst(false);
+ensures Size(Y) == Size(X) + Size(MapDiff(Y, X));
+
+procedure {:yields} {:layer 0} {:refines "atomic_DecrementFreeSpace"} DecrementFreeSpace({:linear "tid"} tid: Tid);
+
+procedure {:atomic} {:layer 1} atomic_DecrementFreeSpace({:linear "tid"} tid: Tid)
+modifies freeSpace, allocMap;
 {
-    yield;
-    assert {:layer 1} mutatorAddr(tid);
-    assert {:layer 1} Invariant(NumFreeAtOrAfter, AllocatingAtOrAfter, Free, freeSpace);
-    assert {:layer 1} (forall u: int :: {AllocatingAtOrAfter[u][tid]} AllocatingAtOrAfter[u][tid] <==> memLo <= u && u <= i);
+    var ptr: int;
+    assume 0 < freeSpace;
+    assert !domain#Bijection(allocMap)[tid];
+    assert freeSpace == Size(MapDiff(isFree, range#Bijection(allocMap)));
+    assume MapDiff(isFree, range#Bijection(allocMap))[ptr];
+    freeSpace := freeSpace - 1;
+    call allocMap := Reserve(allocMap, tid, ptr);
 }
 
-procedure {:yields} {:layer 1} Malloc({:cnst "tid"} tid: X)
-requires {:layer 1} mutatorAddr(tid);
-requires {:layer 1} Invariant(NumFreeAtOrAfter, AllocatingAtOrAfter, Free, freeSpace);
-requires {:layer 1} (forall u: int :: !AllocatingAtOrAfter[u][tid]);
-ensures {:layer 1} Invariant(NumFreeAtOrAfter, AllocatingAtOrAfter, Free, freeSpace);
-ensures {:layer 1} (forall u: int :: !AllocatingAtOrAfter[u][tid]);
+procedure {:atomic} Reserve(allocMap: Bijection, tid: Tid, ptr: int) returns (allocMap': Bijection) {
+    assert !domain#Bijection(allocMap)[tid];
+    assert !range#Bijection(allocMap)[ptr];
+    assert memAddr(ptr);
+    allocMap' := Bijection(
+                    domain#Bijection(allocMap)[tid := true],
+                    range#Bijection(allocMap)[ptr := true],
+                    tidToPtr#Bijection(allocMap)[tid := ptr],
+                    ptrToTid#Bijection(allocMap)[ptr := tid]);
+}
+
+procedure {:yields} {:layer 0} {:refines "atomic_AllocIfPtrFree"} AllocIfPtrFree({:linear "tid"} tid: Tid, ptr: int) returns (spaceFound:bool);
+
+procedure {:atomic} {:layer 1} atomic_AllocIfPtrFree({:linear "tid"} tid: Tid, ptr: int) returns (spaceFound:bool)
+modifies isFree, allocMap;
+{
+    var tid': Tid;
+    var ptr': int;
+    assert memAddr(ptr);
+    assert isFree[ptr] || memAddr(ptr + 1);
+    assert domain#Bijection(allocMap)[tid];
+    spaceFound := isFree[ptr];
+    if (spaceFound) {
+        isFree[ptr] := false;
+        call allocMap := Alloc(allocMap, tid, ptr);
+    }
+}
+
+procedure {:atomic} Alloc(allocMap: Bijection, tid: Tid, ptr: int) returns (allocMap': Bijection) {
+    var tid': Tid;
+    var ptr': int;
+    assert domain#Bijection(allocMap)[tid];
+    allocMap' := allocMap;
+    if (range#Bijection(allocMap')[ptr]) {
+        // swap
+        tid' := ptrToTid#Bijection(allocMap')[ptr];
+        ptr' := tidToPtr#Bijection(allocMap')[tid];
+        allocMap' := Bijection(
+                        domain#Bijection(allocMap'),
+                        range#Bijection(allocMap'),
+                        tidToPtr#Bijection(allocMap')[tid := ptr][tid' := ptr'],
+                        ptrToTid#Bijection(allocMap')[ptr := tid][ptr' := tid']);
+    }
+    // alloc
+    ptr' := tidToPtr#Bijection(allocMap')[tid];
+    allocMap' := Bijection(
+                    domain#Bijection(allocMap')[tid := false],
+                    range#Bijection(allocMap')[ptr' := false],
+                    tidToPtr#Bijection(allocMap'),
+                    ptrToTid#Bijection(allocMap'));
+}
+
+procedure {:yields} {:layer 0} {:refines "atomic_Reclaim"} Reclaim() returns (ptr: int);
+
+procedure {:atomic} {:layer 1} atomic_Reclaim() returns (ptr: int)
+modifies freeSpace, isFree;
+{
+    assume memAddr(ptr) && !isFree[ptr];
+    freeSpace := freeSpace + 1;
+    isFree[ptr] := true;
+}
+
+procedure {:yields} {:layer 1}
+{:yield_requires "YieldInvariant"}
+{:yield_ensures "YieldInvariant"}
+Malloc({:linear "tid"} tid: Tid)
+requires {:layer 1} !domain#Bijection(allocMap)[tid];
 {
     var i: int;
     var spaceFound: bool;
 
-    call YieldAlloc(tid, 0);
-
-    assert {:layer 1} memAddr(memLo) ==> (forall v: int :: memAddr(v) && memLo <= v ==> Subset(AllocatingAtOrAfter[v], AllocatingAtOrAfter[memLo]));
-    assert {:layer 1} memAddr(memLo) ==> (forall v: int :: memAddr(v) && v <= memLo ==> Subset(AllocatingAtOrAfter[memLo], AllocatingAtOrAfter[v]));
-
     call DecrementFreeSpace(tid);
     i := memLo;
-
-    call YieldAlloc(tid, i);
-
+    call {:layer 1} SizeLemma1(MapDiff(isFree, range#Bijection(allocMap)), tidToPtr#Bijection(allocMap)[tid]);
     while (i < memHi)
-    invariant {:layer 1} memAddr(i);
-    invariant {:layer 1} Invariant(NumFreeAtOrAfter, AllocatingAtOrAfter, Free, freeSpace);
-    invariant {:layer 1} (forall u: int :: AllocatingAtOrAfter[u][tid] <==> memLo <= u && u <= i);
+    invariant {:yields} {:layer 1} memAddr(i) && domain#Bijection(allocMap)[tid] && i <= tidToPtr#Bijection(allocMap)[tid];
+    invariant {:yields} {:layer 1} {:yield_loop "YieldInvariant"} true;
     {
-        assert {:layer 1} memAddr(i+1) ==> (forall v: int :: memAddr(v) && i+1 <= v ==> Subset(AllocatingAtOrAfter[v], AllocatingAtOrAfter[i+1]));
-        assert {:layer 1} memAddr(i+1) ==> (forall v: int :: memAddr(v) && v <= i+1 ==> Subset(AllocatingAtOrAfter[i+1], AllocatingAtOrAfter[v]));
-
+        call {:layer 1} SizeLemma1(isFree, i);
+        call {:layer 1} SizeLemma1(range#Bijection(allocMap), i);
+        call {:layer 1} SizeLemma1(range#Bijection(allocMap), tidToPtr#Bijection(allocMap)[tid]);
+        call {:layer 1} SizeLemma2(range#Bijection(allocMap), isFree);
         call spaceFound := AllocIfPtrFree(tid, i);
-
         if (spaceFound)
         {
-            call YieldAlloc(tid, 0);
+            call {:layer 1} SizeLemma2(range#Bijection(allocMap), isFree);
             return;
         }
-        else
-        {
-            i := i + 1;
-        }
-        call YieldAlloc(tid, i);
+        i := i + 1;
     }
-
-    yield;
     assert {:layer 1} false;
 }
 
-procedure {:yields} {:layer 1} YieldCollect({:cnst "tid"} tid: X)
-requires {:layer 1} tid == GcTid;
-requires {:layer 1} Invariant(NumFreeAtOrAfter, AllocatingAtOrAfter, Free, freeSpace);
-ensures {:layer 1} Invariant(NumFreeAtOrAfter, AllocatingAtOrAfter, Free, freeSpace);
+procedure {:yields} {:layer 1}
+{:yield_requires "YieldInvariant"}
+{:yield_ensures "YieldInvariant"}
+Collect()
 {
-    yield;
-    assert {:layer 1} tid == GcTid;
-    assert {:layer 1} Invariant(NumFreeAtOrAfter, AllocatingAtOrAfter, Free, freeSpace);
-}
-
-procedure {:yields} {:layer 1} Collect({:cnst "tid"} tid: X)
-requires {:layer 1} tid == GcTid;
-requires {:layer 1} Invariant(NumFreeAtOrAfter, AllocatingAtOrAfter, Free, freeSpace);
-ensures {:layer 1} Invariant(NumFreeAtOrAfter, AllocatingAtOrAfter, Free, freeSpace);
-{
-    call YieldCollect(tid);
+    var ptr: int;
 
     while (*)
-    invariant {:layer 1} Invariant(NumFreeAtOrAfter, AllocatingAtOrAfter, Free, freeSpace);
+    invariant {:yields} {:layer 1} {:yield_loop "YieldInvariant"} true;
     {
-        call Reclaim(tid);
-        call YieldCollect(tid);
+        call ptr := Reclaim();
+        call {:layer 1} SizeLemma1(MapDiff(isFree, range#Bijection(allocMap)), ptr);
     }
-    call YieldCollect(tid);
 }
